theories/examples/instr.v
@@ -4,6 +4,8 @@ From HypVeri.rules Require Import rules_base mov str.
 Section instr.
   (* shorthands for writing programs *)
 
+  Context `{hypparams: HypervisorParameters}.
+
   Definition str_I r a := encode_instruction (Str r a).
   Definition mov_word_I ra w := encode_instruction (Mov ra (inl w)).
   Definition halt_I := encode_instruction Halt.
