theories/examples/lending.v
@@ -1,0 +1,155 @@
+From machine_program_logic.program_logic Require Import weakestpre.
+From iris.staging Require Import monotone.
+From HypVeri.algebra Require Import base.
+(* From HypVeri.rules Require Import rules_base. *)
+(* From HypVeri.examples Require Import instr. *)
+From HypVeri Require Import proofmode.
+
+
+
+Section proof.
+
+  Local Program Instance vmconfig : HypervisorConstants :=
+    {vm_count := 2;
+     vm_count_pos:= _}.
+  Solve Obligations with lia.
+
+  Program Definition V0 : VMID := (@nat_to_fin 0 _ _).
+  Solve Obligations with rewrite /vmconfig /=; lia.
+
+  Program Definition V1 : VMID := (@nat_to_fin 1 _ _).
+  Solve Obligations with rewrite /vmconfig /=; lia.
+
+  Context `{hypparams: !HypervisorParameters}.
+
+  (* STSs *)
+  Definition inv_sts_state: Type := VMID * coPset * bool.
+
+  Inductive inv_sts_base: relation inv_sts_state :=
+  | inv_sts_base_0_closed_unchanged_open ι: inv_sts_base (V0, ⊤, false) (V0, ⊤ ∖ ι, false)
+  | inv_sts_base_0_unclosed_unchanged_switch ι: inv_sts_base (V0, ⊤ ∖ ι, false) (V1, ⊤, false)
+  | inv_sts_base_1_closed_unchanged_change ι: inv_sts_base (V1, ⊤, false) (V1, ⊤ ∖ ι, true)
+  | inv_sts_base_1_unclosed_changed_switch ι: inv_sts_base (V1, ⊤ ∖ ι, true) (V0, ⊤, true)
+  | inv_sts_base_0_closed_changed_open ι: inv_sts_base (V0, ⊤, true) (V0, ⊤ ∖ ι, true).
+
+  Definition inv_sts_rel := rtc inv_sts_base.
+
+  Definition nainv_sts_state: Type :=  Word * Word * option handle.
+
+  Inductive nainv_sts_base: relation nainv_sts_state :=
+  | nainv_sts_base_init_run w0 w0' h: nainv_sts_base (w0, w0', None) (of_imm (encode_hvc_func Run), w0', Some h)
+  | nainv_sts_base_lent_yield w0' h: nainv_sts_base (of_imm (encode_hvc_func Run), w0', Some h)
+                                                    (of_imm (encode_hvc_func Run), of_imm (encode_hvc_func Yield), Some h)
+  | nainv_sts_base_relinquished_reclaim h: nainv_sts_base (of_imm (encode_hvc_func Run), of_imm (encode_hvc_func Yield), Some h)
+                                                          (of_imm (encode_hvc_func Run), of_imm (encode_hvc_func Yield), None).
+
+  Definition nainv_sts_rel := rtc nainv_sts_base.
+
+
+
+  (* CMRAs *)
+  Class tokG Σ := tok_G :> inG Σ (exclR unitO).
+  Class invStsG Σ := invSts_G :> inG Σ (authUR (mraUR inv_sts_rel)).
+  Class nainvStsG Σ := nainvSts_G :> inG Σ (authUR (mraUR nainv_sts_rel)).
+
+  Context `{gen_VMG Σ, tokG Σ, invStsG Σ, nainvStsG Σ}.
+
+  Definition inv_state_exact (γ: gname) (s: inv_sts_state):=
+    own γ (● principal inv_sts_rel s).
+
+  Definition inv_state_atleast (γ: gname) (s: inv_sts_state):=
+    own γ (◯ principal inv_sts_rel s).
+
+  Definition nainv_state_exact (γ: gname) (s: nainv_sts_state):=
+    own γ (● principal nainv_sts_rel s).
+
+  Definition nainv_state_atleast (γ: gname) (s: nainv_sts_state):=
+    own γ (◯ principal nainv_sts_rel s).
+
+  Lemma inv_state_alloc s: ⊢|==> ∃ γ, inv_state_exact γ s.
+  Proof. iApply own_alloc; apply auth_auth_valid; done. Qed.
+
+  Lemma inv_state_exact_atleast γ s s':
+    inv_state_exact γ s -∗ inv_state_atleast γ s' -∗ ⌜inv_sts_rel s' s⌝.
+  Proof.
+    iIntros "H1 H2".
+    iDestruct (own_valid_2 with "H1 H2") as %[Hincl ?]%auth_both_valid_discrete.
+    revert Hincl; rewrite principal_included; done.
+  Qed.
+
+  Lemma inv_state_update γ s s' :
+    inv_sts_rel s s' → inv_state_exact γ s ==∗ inv_state_exact γ s'.
+  Proof.
+    intros Hss.
+    iApply own_update.
+    eapply auth_update_auth.
+    apply mra_local_update_grow; done.
+  Qed.
+
+  Lemma inv_state_observe γ s :
+    inv_state_exact γ s ==∗ inv_state_exact γ s ∗ inv_state_atleast γ s.
+  Proof.
+    rewrite /inv_state_exact /inv_state_atleast -own_op.
+    iApply own_update.
+    eapply auth_update_alloc.
+    apply mra_local_update_get_frag; done.
+  Qed.
+
+  Lemma nainv_state_alloc s: ⊢|==> ∃ γ, nainv_state_exact γ s.
+  Proof. iApply own_alloc; apply auth_auth_valid; done. Qed.
+
+  Lemma nainv_state_exact_atleast γ s s':
+    nainv_state_exact γ s -∗ nainv_state_atleast γ s' -∗ ⌜nainv_sts_rel s' s⌝.
+  Proof.
+    iIntros "H1 H2".
+    iDestruct (own_valid_2 with "H1 H2") as %[Hincl ?]%auth_both_valid_discrete.
+    revert Hincl; rewrite principal_included; done.
+  Qed.
+
+  Lemma nainv_state_update γ s s' :
+    nainv_sts_rel s s' → nainv_state_exact γ s ==∗ nainv_state_exact γ s'.
+  Proof.
+    intros Hss.
+    iApply own_update.
+    eapply auth_update_auth.
+    apply mra_local_update_grow; done.
+  Qed.
+
+  Lemma nainv_state_observe γ s :
+    nainv_state_exact γ s ==∗ nainv_state_exact γ s ∗ nainv_state_atleast γ s.
+  Proof.
+    rewrite /nainv_state_exact /nainv_state_atleast -own_op.
+    iApply own_update.
+    eapply auth_update_alloc.
+    apply mra_local_update_get_frag; done.
+  Qed.
+
+  Definition token γ := own γ (Excl ()).
+
+  Lemma token_alloc : ⊢|==> ∃ γ, token γ.
+  Proof. iApply own_alloc; done. Qed.
+
+  Lemma token_excl γ : token γ -∗ token γ -∗ False.
+  Proof. iIntros "H1 H2"; iDestruct (own_valid_2 with "H1 H2") as %?; done. Qed.
+
+  (* invariants *)
+  Definition inv_name := nroot .@ "lending" .@ "inv".
+  Definition nainv_name := nroot .@ "lending" .@ "na".
+
+  Lemma namespace_disjoint: inv_name ## nainv_name.
+  Proof.
+    apply ndot_ne_disjoint.
+    done.
+  Qed.
+
+
+  (* Definition inv_def γ_invm := *)
+  (*   (∃ (i : @VMID vmconfig) P b, <<i>>{ 1%Qp } ∗ nainv_closed P ∗ inv_state_exact γ_invm (i,P,b) )%I. *)
+
+  (*     <<z>>{ 1%Qp } ∗ nainv_closed (⊤ ∖ ↑ι1) ∗ tokI γ1) *)
+  (*     ∨ <<z>>{ 1%Qp } ∗ nainv_closed ⊤ ∗ tokI γ3 *)
+  (*     ∨ <<i>>{ 1%Qp } ∗ nainv_closed ⊤ ∗ tokI γ1 ∗ tokI γ2 )%I. *)
+
+
+
+End proof.
